StrataTest/DDM/Util/Ion.lean
@@ -32,12 +32,26 @@ def testRoundtrip (v : List (Ion SymbolId)) : Bool :=
 #guard testRoundtrip [.bool false, .bool true]
 #guard testRoundtrip [.int 0, .int 1, .int (-1), .int 256, .int (-256)]
 #guard testRoundtrip [.float 1e-3, .float 3]
-#guard testRoundtrip [.decimal ⟨0, 0 ⟩, .decimal ⟨1, 3 ⟩, .decimal ⟨0, 0 ⟩]
+#guard testRoundtrip [.decimal ⟨0, 0⟩]
+#guard testRoundtrip [.decimal ⟨0, 1⟩]
+#guard testRoundtrip [.decimal ⟨0, -1⟩]
+#guard testRoundtrip [.decimal ⟨0,  65⟩]
+#guard (serialize #[.decimal ⟨0, 256⟩]).asHex = "e00100ea520280"
+#guard (serialize #[.decimal ⟨0, -256⟩]).asHex = "e00100ea524280"
+#guard testRoundtrip [.decimal ⟨0,  256⟩]
+#guard testRoundtrip [.decimal ⟨0, -256⟩]
+#guard testRoundtrip [.decimal ⟨258, 0⟩]
+#guard testRoundtrip [.decimal ⟨-258, 0⟩]
+#guard testRoundtrip [.decimal ⟨1, 3⟩]
+
+#guard testRoundtrip [.symbol (.mk 0), .symbol (.mk 1)]
+
 #guard testRoundtrip [.string "", .string "⟨"]
 #guard testRoundtrip [.string "this_is_a_long_name"]
 
-#guard testRoundtrip [.symbol (.mk 0), .symbol (.mk 1)]
+#guard testRoundtrip [.blob <| Strata.ByteArray.zeros 20000]
 #guard testRoundtrip [.list #[], .list #[.int 1]]
+#guard testRoundtrip [.list (Array.ofFn (n := 8000) fun i => .int i.val)]
 #guard testRoundtrip [.sexp #[], .sexp #[.int 1]]
 #guard testRoundtrip [.struct #[], .struct #[(.mk 1, .int 1)]]
 #guard testRoundtrip [.annotation #[.mk 1] (.int 1)]
